Removed semax_func_cons_ext_with_normalization rule; make all works with expection of material staht needs fcf submodule. Tactics in pile not yet fully adapted

mailbox/verif_mailbox_all.v
@@ -15,22 +15,25 @@ Require Import mailbox.verif_mailbox_main.
 Set Bullet Behavior "Strict Subproofs".
 
 Definition extlink := ext_link_prog prog.
-Definition Espec := add_funspecs (Concurrent_Espec unit _ extlink) extlink Gprog.
+Definition Espec := add_funspecs (Concurrent_Espec unit _ extlink) extlink (normalizeFunspecs Gprog).
 Existing Instance Espec.
 
 (* This lemma ties all the function proofs into a single proof for the entire program. *)
 Lemma all_funcs_correct:
-  semax_func Vprog Gprog (Genv.globalenv prog) (prog_funct prog) 
-   ltac:(old_with_library prog Gprog).
-Proof.
-unfold Gprog, prog, prog_funct, main_pre, main_post, prog_vars; simpl.
-repeat (eapply semax_func_cons_ext_vacuous; [reflexivity | reflexivity | LookupID | LookupB |]).
+  semax_func Vprog (normalizeFunspecs Gprog) (Genv.globalenv prog) (prog_funct prog) 
+    ltac:(old_with_library prog (normalizeFunspecs Gprog)).
+Proof. 
+(*unfold Gprog, prog, prog_funct, main_pre, main_post, prog_vars; simpl.*)
+repeat (eapply semax_func_cons_ext_vacuous; [apply compute_list_norepet_e; reflexivity | reflexivity | reflexivity | LookupID | LookupB |]).
 repeat semax_func_cons_ext.
-semax_func_cons body_malloc. apply semax_func_cons_malloc_aux.
+semax_func_cons body_malloc. 
+{ eapply derives_trans; [ | apply (semax_func_cons_malloc_aux g gx t)].
+  unfold PROPx, LOCALx, local, lift1, liftx, lift; simpl.
+  unfold liftx, lift; simpl. trivial. }
 repeat semax_func_cons_ext.
 { unfold PROPx, LOCALx, local, lift1, liftx, lift; simpl.
   unfold liftx, lift; simpl.
-  Intros; subst.
+  Intros x x0; subst.
   apply prop_right; unfold make_ext_rval, eval_id in *; simpl in *.
   destruct ret; auto. }
 semax_func_cons body_surely_malloc.
@@ -40,10 +43,11 @@ semax_func_cons body_initialize_reader.
 semax_func_cons body_start_read.
 semax_func_cons body_finish_read.
 semax_func_cons body_initialize_writer.
-eapply semax_func_cons; [ reflexivity
+semax_func_cons body_start_write.
+(*eapply semax_func_cons; [ reflexivity
            | repeat apply Forall_cons; try apply Forall_nil; simpl; auto; computable
            | unfold var_sizes_ok; repeat constructor; simpl; computable | reflexivity | LookupID | LookupB 
-           | apply body_start_write |].
+           | apply body_start_write |].*)
 semax_func_cons body_finish_write.
 semax_func_cons body_reader.
 semax_func_cons body_writer.
