floyd/forward_lemmas.v
@@ -25,6 +25,73 @@ Proof. induction l; simpl; intros; destruct t; trivial; inv L.
   simpl; rewrite IHl; trivial.
 Qed.
 
+Lemma length_zip_with_tl {A} (l:list A): forall t (L: length l = length (typelist2list t)),
+      length (zip_with_tl l t) = length l.
+Proof. induction l; simpl; trivial; intros. destruct t; inv L. simpl. rewrite IHl; trivial. Qed.
+
+Lemma map_fst_zip_with_tl {A} (l:list A): forall t (L: length l = length (typelist2list t)), 
+      l = map fst (zip_with_tl l t).
+Proof. induction l; simpl; trivial; intros. destruct t; inv L. simpl; f_equal; eauto. Qed.
+
+Lemma semax_func_cons_ext_vacuous:
+     forall {Espec: OracleKind} (V : varspecs) (G : funspecs) (C : compspecs) ge
+         (fs : list (ident * Clight.fundef)) (id : ident) (ef : external_function)
+         (argsig : typelist) (retsig : type)
+         (G' : funspecs) cc b
+       (LNR: list_norepet (map fst (fst (funsig_of_fundef(External ef argsig retsig cc))))),
+       (id_in_list id (map fst fs)) = false ->
+       ef_sig ef =
+       {|
+         sig_args := typlist_of_typelist (type_of_params (arglist 1 argsig));
+         sig_res := opttyp_of_type retsig;
+         sig_cc := cc_of_fundef (External ef argsig retsig cc) |} ->
+       Genv.find_symbol ge id = Some b ->
+       Genv.find_funct_ptr ge b = Some (External ef argsig retsig cc) ->
+       semax_func V G ge fs G' ->
+       semax_func V G ge ((id, External ef argsig retsig cc) :: fs)
+         ((id, vacuous_funspec (External ef argsig retsig cc)) :: G').
+Proof. intros.
+remember (funsig_of_fundef (External ef argsig retsig cc)) as sig.
+destruct sig as [params retty]. simpl in Heqsig; inv Heqsig.
+remember (normalparams (length (arglist 1 argsig))) as nids.
+remember (zip_with_tl nids (type_of_params (arglist 1 argsig)) ) as nparams.
+
+assert (L: length (map fst (arglist 1 argsig)) = length (typelist2list argsig)).
+{ forget 1%positive as i.
+  clear.
+  revert i; induction argsig; simpl; intros; auto. }
+assert (T: type_of_params (arglist 1 argsig) = argsig).
+{ forget 1%positive as i.
+  clear.
+  revert i; induction argsig; simpl; intros; auto. f_equal. auto. }
+assert (A: map snd (arglist 1 argsig) = typelist2list argsig).
+{ forget 1%positive as i.
+  clear.
+  revert i; induction argsig; simpl; intros; auto. f_equal. auto. }
+assert (N: nparams = zip_with_tl (normalparams (length (arglist 1 argsig))) (type_of_params (arglist 1 argsig))) by (subst; trivial).
+
+specialize (@semax_func_cons_ext Espec V G C ge fs id ef argsig retsig
+  (rmaps.ConstType Impossible) (fun _ _ => FF) (fun _ _ => FF) ). simpl. 
+intros HH; eapply HH; clear HH; try assumption.
+* unfold ident in *. rewrite <-  N. reflexivity.
+* simpl. rewrite Heqnids in Heqnparams; rewrite <- Heqnparams. unfold funspec_normalized. simpl.
+  specialize (semax.zip_with_normalized_normal argsig). rewrite Heqnparams, T.
+  rewrite map_length in L; rewrite L; trivial.
+* rewrite T, <- Heqnids. f_equal. rewrite Heqnparams, T. apply map_fst_zip_with_tl. 
+  rewrite Heqnids, length_normalparams, <- L, map_length; trivial. 
+* rewrite H0. f_equal. f_equal. rewrite T at 2.
+  apply semax_call.map_snd_typeof_params. rewrite snd_zip_with_tl. apply A.
+  rewrite length_normalparams, <- L, map_length; trivial. 
+* rewrite <- L, ! map_length, Heqnparams. rewrite length_zip_with_tl.
+  + rewrite Heqnids, length_normalparams; trivial.
+  + rewrite T, <- L, Heqnids, length_normalparams, map_length; trivial. 
+* right. clear. hnf. intros. simpl in X; inv X.
+* intros. simpl. apply andp_left1, FF_left.
+* eassumption.
+* assumption.
+* apply semax_external_FF.
+Qed. 
+(* Proof using semax_func_cons_ext_with_normalization 
 Lemma semax_func_cons_ext_vacuous:
      forall {Espec: OracleKind} (V : varspecs) (G : funspecs) (C : compspecs) ge
          (fs : list (ident * Clight.fundef)) (id : ident) (ef : external_function)
@@ -75,7 +142,7 @@ apply H4; clear H4 N; trivial.
 * right. clear. hnf. intros. destruct X.
 * intros. simpl. apply andp_left1, FF_left.
 * apply semax_external_FF.
-Qed.
+Qed.*)
 
 Lemma int_eq_false_e:
   forall i j, Int.eq i j = false -> i <> j.
